mm2 progress

MM2_rev.v
@@ -11,12 +11,26 @@ Proof.
   move=> m /= <-. by have ->: n + S m = S n + m by lia.
 Qed.
 
+Section ForallNorm.
+Context {X : Type} {P : X -> Prop}.
+
+Lemma ForallE {l} : Forall P l -> if l is x :: l then P x /\ Forall P l else True.
+Proof. by case. Qed.
+End ForallNorm.
+Lemma Forall_mapP {X Y : Type} {P : Y -> Prop} {f : X -> Y} {l : list X} : 
+  Forall P (map f l) <-> Forall (fun x => P (f x)) l.
+Proof.
+  elim: l; [constructor; by constructor | ].
+  move=> ? ? IH /=. constructor => /ForallE [? /IH ?]; by constructor.
+Qed.
+
 Section DECIDRE.
 
 Variable M : Mm2.
 
 Notation step := (MM2.step M).
 Notation multi_step := (MM2.multi_step M).
+Notation terminating := (MM2.terminating M).
 Notation l := (length M).
 
 (* 
@@ -26,6 +40,7 @@ Notation l := (length M).
   - a small configuration (both counter < l )
   - a configuration where one of the counters is 0 and the other did not decrease much
 *)
+
 Lemma next_waypoint p a b :
   (exists k, 0 < k <= l - p + 1 /\ 
     match multi_step k (p, (a, b)) with
@@ -83,3 +98,265 @@ Proof.
       case: (multi_step k (S p, (a, b))) Hk; last done.
       move=> [? [? ?]]. lia.
 Qed.
+
+Lemma multi_step_ubound {k p a b p' a' b'} : multi_step k (p, (a, b)) = Some (p', (a', b')) -> a' <= k + a /\ b' <= k + b.
+Proof.
+Admitted.
+
+Lemma iter_None {X : Type} (f : X -> option X) k : Nat.iter k (option_bind f) None = None.
+Proof. elim: k; [done | by move=> /= ? ->]. Qed.
+
+Lemma option_bind_iter {X : Type} (f : X -> option X) k x : 
+  option_bind f (Nat.iter k (option_bind f) (Some x)) = Nat.iter k (option_bind f) (f x).
+Proof. elim: k; [done|by move=> k /= ->]. Qed.
+
+(* parallel run *)
+Lemma parallel_b {k p a b p' a' b'} : multi_step k (p, (a, b)) = Some (p', (a', b')) -> k < b ->
+  (exists k' p'' a'', k' <= k /\ multi_step k' (p, (a, b)) = Some (p'', (a'', 0))) \/
+  forall n, multi_step k (p, (a, n+b)) = Some (p', (a', n+b')).
+Proof.
+  elim: k p a b.
+  { move=> p a b /= [] *. subst. by right. }
+  move=> k IH p a b.
+  rewrite /= option_bind_iter.
+  rewrite /step. case Hi: (nth_error M (state (p, (a, b)))) => [i|]; last by rewrite iter_None.
+  rewrite -/step. case: i Hi.
+  - by rewrite iter_None.
+  - case.
+    + (* zero b *)
+      move=> /= Hi ? ?. left. exists 1, (S p), a.
+      split; first by lia. by rewrite /= /step Hi.
+    + (* zero a *)
+      move=> /= Hi /IH {}IH ?.
+      have /IH [[k' [p'' [a'' [? H]]]]|] : k < b by lia.
+      * left. exists (S k'), p'', a''. split; first by lia.
+        have -> : S k' = 1 + k' by lia. rewrite /(multi_step (1+k')) iter_plus /=.
+        by rewrite /step Hi /= -/step -H.
+      * move=> H. right. move=> k'. by rewrite option_bind_iter /step Hi -/step -H.
+  Admitted.
+
+Lemma parallel_a {k p a b p' a' b'} : multi_step k (p, (a, b)) = Some (p', (a', b')) -> k < a ->
+  (exists k' p'' b'', k' <= k /\ multi_step k' (p, (a, b)) = Some (p'', (0, b''))) \/
+  forall n, multi_step k (p, (n+a, b)) = Some (p', (n+a', b')).
+Proof. Admitted.
+
+(*
+(* todo needs waypoint after l not l+1 steps? or small bound set to l+1? *)
+Corollary next_waypoint_b p b : b > l + 1 ->
+  (exists k, 0 < k <= l + 1 /\ 
+    (multi_step k (p, (0, b)) = None \/
+    (exists p' b', multi_step k (p, (0, b)) = Some (p', (0, b')) /\ b <= b' + l) \/
+    exists p' a' b', multi_step k (p, (0, b)) = Some (p', (a', b')) /\ a' <= l + 1 /\ b' <= l + 1)).
+Proof.
+  move=> ?. have [k [? Hk]] := next_waypoint p 0 b.
+  exists k. split; first by lia.
+  move: Hk. case E: (multi_step k (p, (0, b))) => [[p' [a' b']]|]; last by tauto.
+  move=> [?|[?|?]]; right.
+  - right. exists p', a', b'. split; [done|lia].
+  - left. exists p', b'. split; last by lia.
+    congr (Some (p', (_, b'))). tauto.
+  - have [?|?] : a' <= l + 1 \/ l + 1 < a' by lia.
+    + right. exists p', a', 0. split; last by lia.
+      congr (Some (p', (a', _))). tauto.
+    + have := asd E. lia.
+Qed.
+*)
+
+Definition reaches (x y: Config) := exists k, multi_step k x = Some y.
+Definition reaches_plus (x y: Config) := exists k, 0 < k /\ multi_step k x = Some y.
+Definition non_terminating x := forall k, multi_step k x <> None.
+
+(* terminate or reach uniformly next config or reach small config *)
+Corollary next_waypoint_b p b :
+  terminating (p, (0, b)) \/
+  (exists p' b', forall n, reaches_plus (p, (0, n+b)) (p', (0, n+b'))) \/
+  exists p' a' b', reaches (p, (0, b)) (p', (a', b')) /\ a' <= l + 1 /\ b' <= l + 1.
+Proof.
+  have [?|?] : b <= l + 1 \/ b > l + 1 by lia.
+  { do 2 right. exists p, 0, b. split; [by exists 0 | lia]. }
+  have [k [? Hk]] := next_waypoint p 0 b.
+  move: Hk. case E: (multi_step k (p, (0, b))) => [[p' [a' b']]|]; first last.
+  { move=> _. left. by exists k. }
+  move=> [?|[?|?]]; right.
+  - right. exists p', a', b'. split; [|lia]. by exists k.
+  - move: E => /parallel_b => /(_ ltac:(lia)) [].
+    + move=> [k' [p'' [a'' [?]]]] Hk'.
+      move: (Hk') => /multi_step_ubound ?. right.
+      exists p'', a'', 0. split; last by lia.
+      by exists k'.
+    + move=> H. left. exists p', b' => n. exists k. split; first by lia.
+      rewrite (H n). congr (Some (p', (_, n + b'))). lia.
+  - right. exists p', a', 0.
+    move: (E) => /multi_step_ubound ?.
+    split; last by lia.
+    exists k. rewrite E. congr (Some (p', (a', _))). lia.
+Qed.
+
+(*
+Corollary next_waypoint_a p a : a > l + 1 ->
+  (exists k, 0 < k <= l + 1 /\ 
+    (multi_step k (p, (a, 0)) = None \/
+    (exists p' a', multi_step k (p, (a, 0)) = Some (p', (a', 0)) /\ a <= a' + l) \/
+    exists p' a' b', multi_step k (p, (a, 0)) = Some (p', (a', b')) /\ a' <= l + 1 /\ b' <= l + 1)).
+Proof.
+  move=> ?. have [k [? Hk]] := next_waypoint p a 0.
+  exists k. split; first by lia.
+  move: Hk. case E: (multi_step k (p, (a, 0))) => [[p' [a' b']]|]; last by tauto.
+  move=> [?|[?|?]]; right.
+  - right. exists p', a', b'. split; [done|lia].
+  - have [?|?] : b' <= l + 1 \/ l + 1 < b' by lia.
+    + right. exists p', 0, b'. split; last by lia.
+      congr (Some (p', (_, b'))). tauto.
+    + have := asd E. lia.
+  - left. exists p', a'. split; last by lia.
+    congr (Some (p', (a', _))). tauto.
+Qed.
+*)
+
+
+Lemma distinct_states x L :
+  Forall (fun y => reaches x y) L -> NoDup (map state L) -> length L <= l+l+2.
+Proof.
+  move=> /Forall_forall HL.
+  suff : incl (map state L) ([state x] ++ (seq 0 (l+1)) ++ (map (fun i => if i is dec _  q then q else 0) M)).
+  { move=> /NoDup_incl_length H /H. rewrite ?app_length ?map_length seq_length /=. lia. }
+  move=> p' /in_map_iff [y [<-]] /HL [[|k]].
+  { move=> /= [->]. by left. }
+  move=> /=. case: (multi_step k x); last done.
+  move=> [p [a b]]. rewrite /= /step.
+  case Hi: (nth_error M (state (p, (a, b)))) => [i|]; last done.
+  have ? : p < l by (apply /nth_error_Some; move: Hi => /= ->).
+  case: i Hi.
+  - done.
+  - move=> ? _ [<-] /=. right. apply /in_app_iff. left. apply /in_seq. lia.
+  - move=> ? _ [<-] /=. right. apply /in_app_iff. left. apply /in_seq. lia.
+  - move=> [] q /= Hi.
+    + move: b => [|b].
+      * move=> [<-] /=. right. apply /in_app_iff. right. apply /in_map_iff.
+        exists (dec true q). split; first done. apply /nth_error_In. eassumption.
+      * move=> [<-] /=. right. apply /in_app_iff. left. apply /in_seq. lia.
+    + move: a => [|a].
+      * move=> [<-] /=. right. apply /in_app_iff. right. apply /in_map_iff.
+        exists (dec false q). split; first done. apply /nth_error_In. eassumption.
+      * move=> [<-] /=. right. apply /in_app_iff. left. apply /in_seq. lia.
+Qed.
+
+Lemma reaches_plus_reaches {x y z} : reaches_plus x y -> reaches y z -> reaches_plus x z.
+Proof.
+  move=> [k [? Hk]] [k' Hk']. exists (k+k'). split; first by lia.
+  move: Hk. by rewrite /multi_step iter_plus => ->.
+Qed.
+
+Lemma reaches_reaches_plus {x y z} : reaches x y -> reaches_plus y z -> reaches_plus x z.
+Proof.
+  move=> [k Hk] [k' [? Hk']]. exists (k+k'). split; first by lia.
+  move: Hk. by rewrite /multi_step iter_plus => ->.
+Qed.
+
+Lemma reaches_plus_incl {x y} : reaches_plus x y -> reaches x y.
+Proof. move=> [k [? Hk]]. by exists k. Qed.
+
+Lemma reaches_terminating {x y} : reaches x y -> terminating y -> terminating x.
+Proof.
+  move=> [k Hk] [k' Hk']. exists (k+k').
+  move: Hk. by rewrite /multi_step iter_plus => ->.
+Qed.
+
+Lemma reaches_non_terminating {x y} : reaches x y -> non_terminating y -> non_terminating x.
+Proof.
+  move=> [k Hk] Hy k' Hk'.
+Admitted.
+
+Lemma reaches_trans {x y z} : reaches x y -> reaches y z -> reaches x z.
+Proof. Admitted.
+
+Lemma big p b p' b' (L : list (nat*nat)) :
+  0 < length L -> 
+  NoDup (map fst L) ->
+  Forall (fun '(p'', b'') => forall n, reaches (p, (0, n+b)) (p'', (0, n+b''))) L ->
+  Forall (fun '(p'', b'') => forall n, reaches (p'', (0, n+b'')) (p', (0, n+b'))) L -> 
+  terminating (p, (0, b)) \/
+  non_terminating (p, (0, b)) \/
+  (exists p'' a'' b'', reaches (p, (0, b)) (p'', (a'', b'')) /\ a'' <= l + 1 /\ b'' <= l + 1).
+Proof.
+  move Hn: ((l+l+3) - length L) => n.
+  elim: n L Hn p' b'.
+  { move=> L ? p' b' _ H1L. move: (H1L) => /NoDup_incl_length H H2L.
+    pose L' := map (fun '(p'', b'') => (p'', (0, b''))) L.
+    suff : length L' <= l+l+2 by (rewrite /L' map_length; lia).
+    apply /(distinct_states (p, (0, b))).
+    - rewrite /L' Forall_mapP. apply: Forall_impl H2L.
+      by move=> [p'' b''] /(_ 0).
+    - rewrite /L' map_map. move: H1L. congr NoDup.
+      by apply /map_ext => - [? ?]. }
+  move=> k IH L ? p' b' H0L H1L H2L H3L.
+  have H : forall n, reaches (p, (0, n+b)) (p', (0, n+b')).
+  { move: H0L H2L H3L. clear. case: L => /=; first by lia.
+    move=> [p'' b''] ? _ /ForallE [H1 _] /ForallE [H2 _] n.
+    exact: (reaches_trans (H1 n) (H2 n)). }
+  have [H1|[[p'' [b'' H2]]|[p'' [a'' [b'' [H3 ?]]]]]] := next_waypoint_b p' b'.
+  - left. exact: (reaches_terminating (H 0) H1).
+  - have [|Hp''] := In_dec Nat.eq_dec p'' (map fst L).
+    + (* state visited *)
+      move=> /in_map_iff [[p''' b'''] /= [?]] H4L. subst p'''.
+      move: H2L (H4L) => /Forall_forall H' /H'{H'} H2L.
+      move: H3L (H4L) => /Forall_forall H' /H'{H'} H3L.
+      have [?|?] : b''' <= b'' \/ b'' < b''' by lia.
+      * right. left. apply: (reaches_non_terminating (H 0)).
+        apply: (reaches_non_terminating (reaches_plus_incl (H2 0))).
+        have H' : forall n, reaches_plus (p'', (0, n + b''')) (p'', (0, n + b'')).
+        { move=> n. exact: (reaches_reaches_plus (H3L n) (H2 n)). }
+        move=> k'. admit. (* doable via loop *)
+      * do 2 right. exists p'', 0. (* HOW TO GO DOWN? *)
+    + (* state not visited *)
+      have := IH ((p'', b'') :: L).
+      move=> /= /(_ ltac:(lia) p'' b''). apply.
+      * lia.
+      * by constructor.
+      * constructor; last done.
+        move=> n. exact: (reaches_trans (H n) (reaches_plus_incl (H2 n))).
+      * constructor.
+        { move=> n. by exists 0. }
+        apply: Forall_impl H3L => - [p''' b'''] H' n.
+        exact: (reaches_trans (H' n) (reaches_plus_incl (H2 n))).
+  - do 2 right. exists p'', a'', b''. split; last done.
+    exact: (reaches_trans (H 0) H3).
+Admitted.
+
+(* not enough 
+Lemma big p b p' b' (L : list (nat*nat)) :
+  (forall n, reaches_plus (p, (0, n+b)) (p', (0, n+b'))) ->
+  NoDup (map fst L) ->
+  Forall (fun '(p'', b'') => forall n, reaches (p, (0, n+b)) (p'', (0, n+b''))) L -> 
+  terminating (p, (0, b)) \/
+  non_terminating (p, (0, b)) \/
+  (exists p'' a'' b'', reaches_plus (p, (0, b)) (p'', (a'', b'')) /\ a'' <= l + 1 /\ b'' <= l + 1).
+Proof.
+  move Hn: ((l+l+3) - length L) => n.
+  elim: n L Hn p' b'.
+  { move=> L ? p' b' ? H1L. move: (H1L) => /NoDup_incl_length H H2L.
+    pose L' := map (fun '(p'', b'') => (p'', (0, b''))) L.
+    suff : length L' <= l+l+2 by (rewrite /L' map_length; lia).
+    apply /(distinct_states (p, (0, b))).
+    - rewrite /L' Forall_mapP. apply: Forall_impl H2L.
+      by move=> [p'' b''] /(_ 0).
+    - rewrite /L' map_map. move: H1L. congr NoDup.
+      by apply /map_ext => - [? ?]. }
+  move=> k IH L ? p' b' H H1L H2L.
+  have [H1|[[p'' [b'' H2]]|[p'' [a'' [b'' [H3 ?]]]]]] := next_waypoint_b p' b'.
+  - left. exact: (reaches_terminating (reaches_plus_incl (H 0)) H1).  (* easy *)
+  - have [|Hp''] := In_dec Nat.eq_dec p'' (map fst L).
+    + (* state visited *)
+      move=> /in_map_iff [[p''' b'''] /= [?]]. subst p'''.
+      move: H2L => /Forall_forall H' /H'{H'}.
+    + (* state not visited *)
+      have := IH ((p'', b'') :: L).
+      move=> /= /(_ ltac:(lia) p'' b''). apply.
+      * move=> n. exact: (reaches_plus_reaches (H n) (reaches_plus_incl (H2 n))).
+      * by constructor.
+      * constructor; last done.
+        move=> n. exact: (reaches_plus_incl (reaches_plus_reaches (H n) (reaches_plus_incl (H2 n)))).
+  - do 2 right. exists p'', a'', b''. split; last done.
+    exact: (reaches_plus_reaches (H 0) H3).
+Admitted.
+*)
